<?xml version="1.0"?>
<rdf:RDF xmlns="http://www.semanticweb.org/victor/ontologies/2023/8/18/untitled-ontology-57#"
     xml:base="http://www.semanticweb.org/victor/ontologies/2023/8/18/untitled-ontology-57"
     xmlns:owl="http://www.w3.org/2002/07/owl#"
     xmlns:rdf="http://www.w3.org/1999/02/22-rdf-syntax-ns#"
     xmlns:xml="http://www.w3.org/XML/1998/namespace"
     xmlns:xsd="http://www.w3.org/2001/XMLSchema#"
     xmlns:rdfs="http://www.w3.org/2000/01/rdf-schema#">
    <owl:Ontology rdf:about="http://purl.org/ontology/TextualReknittings">
        <rdfs:comment>Ontology of the Textual Reknittings Workshop as part of Victor Chaix&apos;s Master thesis in Digitial Humanities and Digital Knowledge, at the University of Bologna</rdfs:comment>
        <rdfs:label>TextualReknittingsOntology</rdfs:label>
        <owl:versionInfo rdf:datatype="http://www.w3.org/2001/XMLSchema#integer">2023</owl:versionInfo>
    </owl:Ontology>
    


    <!-- 
    ///////////////////////////////////////////////////////////////////////////////////////
    //
    // Annotation properties
    //
    ///////////////////////////////////////////////////////////////////////////////////////
     -->

    


    <!-- http://www.w3.org/1999/02/22-rdf-syntax-ns#dctitle -->

    <owl:AnnotationProperty rdf:about="http://www.w3.org/1999/02/22-rdf-syntax-ns#dctitle">
        <rdfs:subPropertyOf rdf:resource="http://www.w3.org/2002/07/owl#backwardCompatibleWith"/>
    </owl:AnnotationProperty>
    


    <!-- 
    ///////////////////////////////////////////////////////////////////////////////////////
    //
    // Object Properties
    //
    ///////////////////////////////////////////////////////////////////////////////////////
     -->

    


    <!-- http://purl.org/dc/terms/creator -->

    <owl:ObjectProperty rdf:about="http://purl.org/dc/terms/creator">
        <rdfs:domain rdf:resource="http://purl.org/ontology/TextualReknittings/Text"/>
        <rdfs:range rdf:resource="http://purl.org/ontology/TextualReknittings/Individuator"/>
    </owl:ObjectProperty>
    


    <!-- http://purl.org/ontology/TextualReknittings/chosenBy -->

    <owl:ObjectProperty rdf:about="http://purl.org/ontology/TextualReknittings/chosenBy">
        <rdfs:subPropertyOf rdf:resource="http://www.w3.org/2002/07/owl#topObjectProperty"/>
        <rdfs:domain rdf:resource="http://purl.org/ontology/TextualReknittings/InitialText"/>
        <rdfs:range rdf:resource="http://purl.org/ontology/TextualReknittings/Group"/>
    </owl:ObjectProperty>
    


    <!-- http://purl.org/ontology/TextualReknittings/hasCategories -->

    <owl:ObjectProperty rdf:about="http://purl.org/ontology/TextualReknittings/hasCategories">
        <rdfs:subPropertyOf rdf:resource="http://www.w3.org/2002/07/owl#topObjectProperty"/>
        <rdfs:domain rdf:resource="http://purl.org/ontology/TextualReknittings/RefragmentedWiki"/>
        <rdfs:range rdf:resource="http://purl.org/ontology/TextualReknittings/Tag"/>
    </owl:ObjectProperty>
    


    <!-- http://purl.org/ontology/TextualReknittings/hasComment -->

    <owl:ObjectProperty rdf:about="http://purl.org/ontology/TextualReknittings/hasComment">
        <rdfs:domain rdf:resource="http://purl.org/ontology/TextualReknittings/TextAnnotation"/>
        <rdfs:range rdf:resource="http://purl.org/ontology/TextualReknittings/TextAnnotation"/>
    </owl:ObjectProperty>
    


    <!-- http://www.purl.org/ontology/TextualReknittings/hasTag -->

    <owl:ObjectProperty rdf:about="http://www.purl.org/ontology/TextualReknittings/hasTag">
        <rdfs:domain rdf:resource="http://purl.org/ontology/TextualReknittings/TextAnnotation"/>
        <rdfs:range rdf:resource="http://purl.org/ontology/TextualReknittings/Tag"/>
    </owl:ObjectProperty>
    


    <!-- 
    ///////////////////////////////////////////////////////////////////////////////////////
    //
    // Data properties
    //
    ///////////////////////////////////////////////////////////////////////////////////////
     -->

    


    <!-- http://purl.org/ontology/TextualReknittings/containsText -->

    <owl:DatatypeProperty rdf:about="http://purl.org/ontology/TextualReknittings/containsText">
        <rdfs:domain rdf:resource="http://purl.org/ontology/TextualReknittings/TextAnnotation"/>
        <rdfs:range rdf:resource="http://www.w3.org/2000/01/rdf-schema#Literal"/>
        <rdfs:comment>The text that is included in an annotation.</rdfs:comment>
    </owl:DatatypeProperty>
    


    <!-- http://purl.org/ontology/TextualReknittings/hasSource -->

    <owl:DatatypeProperty rdf:about="http://purl.org/ontology/TextualReknittings/hasSource">
        <rdfs:domain rdf:resource="http://purl.org/ontology/TextualReknittings/InitialText"/>
        <rdfs:range rdf:resource="http://www.w3.org/2000/01/rdf-schema#Literal"/>
        <rdfs:comment>The URL of the web text that has been read.</rdfs:comment>
    </owl:DatatypeProperty>
    


    <!-- 
    ///////////////////////////////////////////////////////////////////////////////////////
    //
    // Classes
    //
    ///////////////////////////////////////////////////////////////////////////////////////
     -->

    


    <!-- http://purl.org/ontology/TextualReknittings/Affection -->

    <owl:Class rdf:about="http://purl.org/ontology/TextualReknittings/Affection">
        <rdfs:subClassOf rdf:resource="http://purl.org/ontology/TextualReknittings/Tag"/>
        <rdfs:comment>What is appreciated, well formulated, touches the emotions.</rdfs:comment>
    </owl:Class>
    


    <!-- http://purl.org/ontology/TextualReknittings/Annotator -->

    <owl:Class rdf:about="http://purl.org/ontology/TextualReknittings/Annotator">
        <rdfs:subClassOf rdf:resource="http://purl.org/ontology/TextualReknittings/Individual"/>
        <owl:disjointWith rdf:resource="http://purl.org/ontology/TextualReknittings/Categorizer"/>
        <owl:disjointWith rdf:resource="http://purl.org/ontology/TextualReknittings/Curator"/>
        <rdfs:comment>Individual that has annotated or replied to annotations over texts of the digital social reading experiment.</rdfs:comment>
    </owl:Class>
    


    <!-- http://purl.org/ontology/TextualReknittings/Approval -->

    <owl:Class rdf:about="http://purl.org/ontology/TextualReknittings/Approval">
        <rdfs:subClassOf rdf:resource="http://purl.org/ontology/TextualReknittings/Tag"/>
        <rdfs:comment>What is agreed upon, fits into preconceptions.</rdfs:comment>
    </owl:Class>
    


    <!-- http://purl.org/ontology/TextualReknittings/Categorizer -->

    <owl:Class rdf:about="http://purl.org/ontology/TextualReknittings/Categorizer">
        <rdfs:subClassOf rdf:resource="http://purl.org/ontology/TextualReknittings/Individual"/>
        <rdfs:comment>The individual responsible for the further tagging of the rewritten output in a wiki format, so that fragments of the output can also serve as an organized and categorized archive for the group.</rdfs:comment>
    </owl:Class>
    


    <!-- http://purl.org/ontology/TextualReknittings/Citation -->

    <owl:Class rdf:about="http://purl.org/ontology/TextualReknittings/Citation">
        <rdfs:subClassOf rdf:resource="http://purl.org/ontology/TextualReknittings/Tag"/>
        <rdfs:comment>What strikes out as important external material/reference, supports an idea.</rdfs:comment>
    </owl:Class>
    


    <!-- http://purl.org/ontology/TextualReknittings/Commentary -->

    <owl:Class rdf:about="http://purl.org/ontology/TextualReknittings/Commentary">
        <rdfs:subClassOf rdf:resource="http://purl.org/ontology/TextualReknittings/Tag"/>
        <rdfs:comment>wWhat is missing from the textual information and should be added.</rdfs:comment>
    </owl:Class>
    


    <!-- http://purl.org/ontology/TextualReknittings/Curator -->

    <owl:Class rdf:about="http://purl.org/ontology/TextualReknittings/Curator">
        <rdfs:subClassOf rdf:resource="http://purl.org/ontology/TextualReknittings/Individual"/>
        <rdfs:comment>The individual that is responsible for coordinating the digital social reading experiment, by animating it and by specifying to the participants the different tags, practices and goals.</rdfs:comment>
    </owl:Class>
    


    <!-- http://purl.org/ontology/TextualReknittings/Disapproval -->

    <owl:Class rdf:about="http://purl.org/ontology/TextualReknittings/Disapproval">
        <rdfs:subClassOf rdf:resource="http://purl.org/ontology/TextualReknittings/Tag"/>
        <rdfs:comment>What is disagreed upon, does not fit into preconceptions.</rdfs:comment>
    </owl:Class>
    


    <!-- http://purl.org/ontology/TextualReknittings/Group -->

    <owl:Class rdf:about="http://purl.org/ontology/TextualReknittings/Group">
        <rdfs:subClassOf rdf:resource="http://purl.org/ontology/TextualReknittings/Individuator"/>
        <rdfs:comment>The &quot;we&quot; that is taking consistency as part of the simultaneous rewriting of the different annotations, made in the reading and annotating part.</rdfs:comment>
    </owl:Class>
    


    <!-- http://purl.org/ontology/TextualReknittings/Important -->

    <owl:Class rdf:about="http://purl.org/ontology/TextualReknittings/Important">
        <rdfs:subClassOf rdf:resource="http://purl.org/ontology/TextualReknittings/Tag"/>
        <rdfs:comment>What supports.</rdfs:comment>
    </owl:Class>
    


    <!-- http://purl.org/ontology/TextualReknittings/Individual -->

    <owl:Class rdf:about="http://purl.org/ontology/TextualReknittings/Individual">
        <rdfs:subClassOf rdf:resource="http://purl.org/ontology/TextualReknittings/Individuator"/>
        <rdfs:comment>Participant to the curation, annotation and further categorization of the output of a digital social reading experiment.</rdfs:comment>
    </owl:Class>
    


    <!-- http://purl.org/ontology/TextualReknittings/Individuator -->

    <owl:Class rdf:about="http://purl.org/ontology/TextualReknittings/Individuator">
        <owl:disjointWith rdf:resource="http://purl.org/ontology/TextualReknittings/Tag"/>
        <owl:disjointWith rdf:resource="http://purl.org/ontology/TextualReknittings/Text"/>
        <rdfs:comment>Individuator consists of the human reader or writer which individuates a text - that is, adds developments to it through annotation and/or rewriting - and concomitantly to this process, individuates itself.</rdfs:comment>
        <rdfs:seeAlso>https://arsindustrialis.org/individuation</rdfs:seeAlso>
    </owl:Class>
    


    <!-- http://purl.org/ontology/TextualReknittings/InitialText -->

    <owl:Class rdf:about="http://purl.org/ontology/TextualReknittings/InitialText">
        <rdfs:subClassOf rdf:resource="http://purl.org/ontology/TextualReknittings/Text"/>
        <owl:disjointWith rdf:resource="http://purl.org/ontology/TextualReknittings/RefragmentedWiki"/>
        <owl:disjointWith rdf:resource="http://purl.org/ontology/TextualReknittings/Rewriting"/>
        <owl:disjointWith rdf:resource="http://purl.org/ontology/TextualReknittings/TextAnnotation"/>
        <rdfs:comment>InitialText is a text chosen by the group to read and annotate collectively, to produce a collective interpretation and appropriation of it for the group&apos;s own goals.</rdfs:comment>
    </owl:Class>
    


    <!-- http://purl.org/ontology/TextualReknittings/Key-word -->

    <owl:Class rdf:about="http://purl.org/ontology/TextualReknittings/Key-word">
        <rdfs:subClassOf rdf:resource="http://purl.org/ontology/TextualReknittings/Tag"/>
        <rdfs:comment>What strikes out as key notions in a text, central to an idea/argument.</rdfs:comment>
    </owl:Class>
    


    <!-- http://purl.org/ontology/TextualReknittings/RefragmentedWiki -->

    <owl:Class rdf:about="http://purl.org/ontology/TextualReknittings/RefragmentedWiki">
        <rdfs:subClassOf rdf:resource="http://purl.org/ontology/TextualReknittings/Text"/>
        <owl:disjointWith rdf:resource="http://purl.org/ontology/TextualReknittings/TextAnnotation"/>
        <rdfs:comment>RefragmentedWiki consists of the further tagging of the rewritten output, in a wiki webpage that separates the different parts of the output as well as the categories of each of its textual fragments. Navigation in the wiki is as such possible through either through the linear parts of the rewritten output or the non-linear tags that have been added to it.</rdfs:comment>
        <rdfs:seeAlso>https://networkcultures.org/reading-group/textual-reknittings/non-linear-output/reports.html</rdfs:seeAlso>
    </owl:Class>
    


    <!-- http://purl.org/ontology/TextualReknittings/Rewriter -->

    <owl:Class rdf:about="http://purl.org/ontology/TextualReknittings/Rewriter">
        <rdfs:subClassOf rdf:resource="http://purl.org/ontology/TextualReknittings/Group"/>
        <rdfs:comment>The rewriter is necessarily a group activity so that the digital social reading experiment becomes a digital social writing one, and for the produced digital social text to reflect a collective interpretation and appropriation of the initial texts.</rdfs:comment>
    </owl:Class>
    


    <!-- http://purl.org/ontology/TextualReknittings/Rewriting -->

    <owl:Class rdf:about="http://purl.org/ontology/TextualReknittings/Rewriting">
        <rdfs:subClassOf rdf:resource="http://purl.org/ontology/TextualReknittings/Text"/>
        <owl:disjointWith rdf:resource="http://purl.org/ontology/TextualReknittings/TextAnnotation"/>
        <rdfs:comment>Rewriting refers to the creative juxtaposition of annotations and their replies, to produce a new text that is a collective interpretation and appropriation of the initial texts.</rdfs:comment>
        <rdfs:seeAlso>https://networkcultures.org/reading-group/textual-reknittings/textual-reknittings.html</rdfs:seeAlso>
    </owl:Class>
    


    <!-- http://purl.org/ontology/TextualReknittings/Tag -->

    <owl:Class rdf:about="http://purl.org/ontology/TextualReknittings/Tag">
        <rdfs:comment>A tag is a meta-categories that has been specified and adopted as part of a digital social reading experiment, to categorize an annotation or annotation-reply. A tag can also serve for a refragmented wiki of a collective rewriting.</rdfs:comment>
    </owl:Class>
    


    <!-- http://purl.org/ontology/TextualReknittings/Text -->

    <owl:Class rdf:about="http://purl.org/ontology/TextualReknittings/Text">
        <rdfs:comment>TextType refers to a different state of the text in the process a digital social text experiment: either an initial chosen text on the web, an annotation or annotation reply, a rewriting of the annotations and selected fragments, or a refragmented wiki of the rewriting output.</rdfs:comment>
        <rdfs:seeAlso>https://hackersanddesigners.nl/s/Summer_Camp_2023/p/Textual_Re-knittings</rdfs:seeAlso>
    </owl:Class>
    


    <!-- http://purl.org/ontology/TextualReknittings/TextAnnotation -->

    <owl:Class rdf:about="http://purl.org/ontology/TextualReknittings/TextAnnotation">
        <rdfs:subClassOf rdf:resource="http://purl.org/ontology/TextualReknittings/Text"/>
        <rdfs:comment>TextAnnotation is a selected fragment in the text that is read, that can be tagged and commented.</rdfs:comment>
        <rdfs:seeAlso>https://networkcultures.org/longform/2023/07/13/hypothes-is-a-story-of-playing-with-digital-texts-expandable-confines/</rdfs:seeAlso>
        <rdfs:seeAlso>https://networkcultures.org/reading-group/textual-reknittings/annotation-archive/all-annotations.html</rdfs:seeAlso>
    </owl:Class>
    


    <!-- http://purl.org/ontology/TextualReknittings/Trouble -->

    <owl:Class rdf:about="http://purl.org/ontology/TextualReknittings/Trouble">
        <rdfs:subClassOf rdf:resource="http://purl.org/ontology/TextualReknittings/Tag"/>
        <rdfs:comment>What suprises.</rdfs:comment>
    </owl:Class>
    


    <!-- 
    ///////////////////////////////////////////////////////////////////////////////////////
    //
    // Individuals
    //
    ///////////////////////////////////////////////////////////////////////////////////////
     -->

    


    <!-- https://w3id.org/arco/ontology/core/Careful_Slugs_vs_Computer_Science -->

    <owl:NamedIndividual rdf:about="https://w3id.org/arco/ontology/core/Careful_Slugs_vs_Computer_Science">
        <rdf:type rdf:resource="http://purl.org/ontology/TextualReknittings/RefragmentedWiki"/>
        <rdf:type rdf:resource="http://purl.org/ontology/TextualReknittings/Rewriting"/>
        <rdfs:comment>Part of the rewriting output and wiki.</rdfs:comment>
        <rdfs:seeAlso>https://networkcultures.org/reading-group/textual-reknittings/textual-reknittings.html#careful-slugs-vs-computer-science</rdfs:seeAlso>
    </owl:NamedIndividual>
    


    <!-- https://w3id.org/arco/ontology/core/Community_and_Infrastructure -->

    <owl:NamedIndividual rdf:about="https://w3id.org/arco/ontology/core/Community_and_Infrastructure">
        <rdf:type rdf:resource="http://purl.org/ontology/TextualReknittings/RefragmentedWiki"/>
        <rdf:type rdf:resource="http://purl.org/ontology/TextualReknittings/Rewriting"/>
        <rdfs:comment>Part of the rewriting output and wiki.</rdfs:comment>
        <rdfs:seeAlso>https://networkcultures.org/reading-group/textual-reknittings/textual-reknittings.html#community-and-infrastructure</rdfs:seeAlso>
    </owl:NamedIndividual>
    


    <!-- https://w3id.org/arco/ontology/core/Drix -->

    <owl:NamedIndividual rdf:about="https://w3id.org/arco/ontology/core/Drix">
        <rdf:type rdf:resource="http://purl.org/ontology/TextualReknittings/Annotator"/>
        <rdf:type rdf:resource="http://purl.org/ontology/TextualReknittings/Individual"/>
        <rdf:type rdf:resource="http://purl.org/ontology/TextualReknittings/Rewriter"/>
        <rdfs:comment>Annotator and participant to the collective rewriting (anonymous).</rdfs:comment>
    </owl:NamedIndividual>
    


    <!-- https://w3id.org/arco/ontology/core/For_Careful_Slugs_Caring_for_Unknowing_in_CS -->

    <owl:NamedIndividual rdf:about="https://w3id.org/arco/ontology/core/For_Careful_Slugs_Caring_for_Unknowing_in_CS">
        <rdf:type rdf:resource="http://purl.org/ontology/TextualReknittings/InitialText"/>
        <rdfs:comment>Chosen initial text.</rdfs:comment>
        <rdfs:seeAlso>https://catalystjournal.org/index.php/catalyst/article/view/37723/30027</rdfs:seeAlso>
    </owl:NamedIndividual>
    


    <!-- https://w3id.org/arco/ontology/core/Planetary_Infrastructure_as_Resistance -->

    <owl:NamedIndividual rdf:about="https://w3id.org/arco/ontology/core/Planetary_Infrastructure_as_Resistance">
        <rdf:type rdf:resource="http://purl.org/ontology/TextualReknittings/InitialText"/>
        <rdfs:comment>Chosen initial text.</rdfs:comment>
        <rdfs:seeAlso>https://zine.zora.co/solarpunk-web3-kareola</rdfs:seeAlso>
    </owl:NamedIndividual>
    


    <!-- https://w3id.org/arco/ontology/core/Selby -->

    <owl:NamedIndividual rdf:about="https://w3id.org/arco/ontology/core/Selby">
        <rdf:type rdf:resource="http://purl.org/ontology/TextualReknittings/Annotator"/>
        <rdf:type rdf:resource="http://purl.org/ontology/TextualReknittings/Individual"/>
        <rdfs:comment>Annotator (not anonymous).</rdfs:comment>
    </owl:NamedIndividual>
    


    <!-- https://w3id.org/arco/ontology/core/Solarpunk_Energy_Imaginaries_and_the_Infrastructures_of_Solidarity -->

    <owl:NamedIndividual rdf:about="https://w3id.org/arco/ontology/core/Solarpunk_Energy_Imaginaries_and_the_Infrastructures_of_Solidarity">
        <rdf:type rdf:resource="http://purl.org/ontology/TextualReknittings/InitialText"/>
        <rdfs:comment>Chosen initial text.</rdfs:comment>
        <rdfs:seeAlso>https://olh.openlibhums.org/article/id/4597/</rdfs:seeAlso>
    </owl:NamedIndividual>
    


    <!-- https://w3id.org/arco/ontology/core/TextualReknittingsWorkshopParticipants -->

    <owl:NamedIndividual rdf:about="https://w3id.org/arco/ontology/core/TextualReknittingsWorkshopParticipants">
        <rdf:type rdf:resource="http://purl.org/ontology/TextualReknittings/Group"/>
        <rdfs:comment>Participants to the workshop in general.</rdfs:comment>
        <rdfs:seeAlso>https://hackersanddesigners.nl/s/Summer_Camp_2023/p/Textual_Re-knittings</rdfs:seeAlso>
    </owl:NamedIndividual>
    


    <!-- https://w3id.org/arco/ontology/core/The_End_of_the_World -->

    <owl:NamedIndividual rdf:about="https://w3id.org/arco/ontology/core/The_End_of_the_World">
        <rdf:type rdf:resource="http://purl.org/ontology/TextualReknittings/RefragmentedWiki"/>
        <rdf:type rdf:resource="http://purl.org/ontology/TextualReknittings/Rewriting"/>
        <rdfs:comment>Part of the rewriting output and wiki.</rdfs:comment>
        <rdfs:seeAlso>https://networkcultures.org/reading-group/textual-reknittings/textual-reknittings.html#the-end-of-the-world</rdfs:seeAlso>
    </owl:NamedIndividual>
    


    <!-- https://w3id.org/arco/ontology/core/VictorChaix -->

    <owl:NamedIndividual rdf:about="https://w3id.org/arco/ontology/core/VictorChaix">
        <rdf:type rdf:resource="http://purl.org/ontology/TextualReknittings/Categorizer"/>
        <rdf:type rdf:resource="http://purl.org/ontology/TextualReknittings/Curator"/>
        <rdf:type rdf:resource="http://purl.org/ontology/TextualReknittings/Individual"/>
        <rdfs:comment>Curator and categorizer (not anonymous).</rdfs:comment>
    </owl:NamedIndividual>
    


    <!-- https://w3id.org/arco/ontology/core/What_is_Solarpunk -->

    <owl:NamedIndividual rdf:about="https://w3id.org/arco/ontology/core/What_is_Solarpunk">
        <rdf:type rdf:resource="http://purl.org/ontology/TextualReknittings/RefragmentedWiki"/>
        <rdf:type rdf:resource="http://purl.org/ontology/TextualReknittings/Rewriting"/>
        <rdfs:comment>Part of the rewriting output and wiki.</rdfs:comment>
        <rdfs:seeAlso>https://networkcultures.org/reading-group/textual-reknittings/textual-reknittings.html#what-is-solar-punk</rdfs:seeAlso>
    </owl:NamedIndividual>
    


    <!-- https://w3id.org/arco/ontology/core/anionet -->

    <owl:NamedIndividual rdf:about="https://w3id.org/arco/ontology/core/anionet">
        <rdf:type rdf:resource="http://purl.org/ontology/TextualReknittings/Annotator"/>
        <rdf:type rdf:resource="http://purl.org/ontology/TextualReknittings/Individual"/>
        <rdfs:comment>Annotator (anonymous).</rdfs:comment>
    </owl:NamedIndividual>
    


    <!-- https://w3id.org/arco/ontology/core/anonymous_onions -->

    <owl:NamedIndividual rdf:about="https://w3id.org/arco/ontology/core/anonymous_onions">
        <rdf:type rdf:resource="http://purl.org/ontology/TextualReknittings/Rewriter"/>
        <rdfs:comment>Participant to the collective rewriting (anonymous).</rdfs:comment>
    </owl:NamedIndividual>
    


    <!-- https://w3id.org/arco/ontology/core/augustomarquet -->

    <owl:NamedIndividual rdf:about="https://w3id.org/arco/ontology/core/augustomarquet">
        <rdf:type rdf:resource="http://purl.org/ontology/TextualReknittings/Annotator"/>
        <rdf:type rdf:resource="http://purl.org/ontology/TextualReknittings/Individual"/>
        <rdfs:comment>Annotator (not anonymous).</rdfs:comment>
    </owl:NamedIndividual>
    


    <!-- https://w3id.org/arco/ontology/core/björn -->

    <owl:NamedIndividual rdf:about="https://w3id.org/arco/ontology/core/björn">
        <rdf:type rdf:resource="http://purl.org/ontology/TextualReknittings/Rewriter"/>
        <rdfs:comment>Participant to the collective rewriting (anonymous).</rdfs:comment>
    </owl:NamedIndividual>
    


    <!-- https://w3id.org/arco/ontology/core/bnjmn -->

    <owl:NamedIndividual rdf:about="https://w3id.org/arco/ontology/core/bnjmn">
        <rdf:type rdf:resource="http://purl.org/ontology/TextualReknittings/Rewriter"/>
        <rdfs:comment>Participant to the collective rewriting (anonymous).</rdfs:comment>
    </owl:NamedIndividual>
    


    <!-- https://w3id.org/arco/ontology/core/cyberfae1312 -->

    <owl:NamedIndividual rdf:about="https://w3id.org/arco/ontology/core/cyberfae1312">
        <rdf:type rdf:resource="http://purl.org/ontology/TextualReknittings/Annotator"/>
        <rdf:type rdf:resource="http://purl.org/ontology/TextualReknittings/Individual"/>
        <rdf:type rdf:resource="http://purl.org/ontology/TextualReknittings/Rewriter"/>
        <rdfs:comment>Annotator and participant to the collective rewriting (anonymous).</rdfs:comment>
    </owl:NamedIndividual>
    


    <!-- https://w3id.org/arco/ontology/core/e -->

    <owl:NamedIndividual rdf:about="https://w3id.org/arco/ontology/core/e">
        <rdf:type rdf:resource="http://purl.org/ontology/TextualReknittings/Rewriter"/>
        <rdfs:comment>Participant to the collective rewriting (anonymous).</rdfs:comment>
    </owl:NamedIndividual>
    


    <!-- https://w3id.org/arco/ontology/core/felixcat -->

    <owl:NamedIndividual rdf:about="https://w3id.org/arco/ontology/core/felixcat">
        <rdf:type rdf:resource="http://purl.org/ontology/TextualReknittings/Annotator"/>
        <rdf:type rdf:resource="http://purl.org/ontology/TextualReknittings/Individual"/>
        <rdf:type rdf:resource="http://purl.org/ontology/TextualReknittings/Rewriter"/>
        <rdfs:comment>Annotator and participant to the collective rewriting (anonymous).</rdfs:comment>
    </owl:NamedIndividual>
    


    <!-- https://w3id.org/arco/ontology/core/goosey -->

    <owl:NamedIndividual rdf:about="https://w3id.org/arco/ontology/core/goosey">
        <rdf:type rdf:resource="http://purl.org/ontology/TextualReknittings/Annotator"/>
        <rdf:type rdf:resource="http://purl.org/ontology/TextualReknittings/Individual"/>
        <rdfs:comment>Annotator (anonymous).</rdfs:comment>
    </owl:NamedIndividual>
    


    <!-- https://w3id.org/arco/ontology/core/hd_onions -->

    <owl:NamedIndividual rdf:about="https://w3id.org/arco/ontology/core/hd_onions">
        <rdf:type rdf:resource="http://purl.org/ontology/TextualReknittings/Annotator"/>
        <rdf:type rdf:resource="http://purl.org/ontology/TextualReknittings/Individual"/>
        <rdfs:comment>Annotator (anonymous).</rdfs:comment>
    </owl:NamedIndividual>
    


    <!-- https://w3id.org/arco/ontology/core/subsignal -->

    <owl:NamedIndividual rdf:about="https://w3id.org/arco/ontology/core/subsignal">
        <rdf:type rdf:resource="http://purl.org/ontology/TextualReknittings/Annotator"/>
        <rdf:type rdf:resource="http://purl.org/ontology/TextualReknittings/Individual"/>
        <rdf:type rdf:resource="http://purl.org/ontology/TextualReknittings/Rewriter"/>
        <rdfs:comment>Annotator (anonymous).</rdfs:comment>
    </owl:NamedIndividual>
    


    <!-- https://w3id.org/arco/ontology/core/-=H=- -->

    <owl:NamedIndividual rdf:about="https://w3id.org/arco/ontology/core/-=H=-">
        <rdf:type rdf:resource="http://purl.org/ontology/TextualReknittings/Rewriter"/>
        <rdfs:comment>Participant to the collective rewriting (anonymous).</rdfs:comment>
    </owl:NamedIndividual>
    


    <!-- https://w3id.org/arco/ontology/core/Solarpunk_&amp;_the_Pedagogical_Value_of_Utopia -->

    <owl:NamedIndividual rdf:about="https://w3id.org/arco/ontology/core/Solarpunk_&amp;_the_Pedagogical_Value_of_Utopia">
        <rdf:type rdf:resource="http://purl.org/ontology/TextualReknittings/InitialText"/>
        <rdfs:comment>Chosen initial text.</rdfs:comment>
        <rdfs:seeAlso>http://www.susted.com/wordpress/content/solarpunk-the-pedagogical-value-of-utopia_2020_05/</rdfs:seeAlso>
    </owl:NamedIndividual>
    


    <!-- 
    ///////////////////////////////////////////////////////////////////////////////////////
    //
    // General axioms
    //
    ///////////////////////////////////////////////////////////////////////////////////////
     -->

    <rdf:Description>
        <rdf:type rdf:resource="http://www.w3.org/2002/07/owl#AllDisjointClasses"/>
        <owl:members rdf:parseType="Collection">
            <rdf:Description rdf:about="http://purl.org/ontology/TextualReknittings/Affection"/>
            <rdf:Description rdf:about="http://purl.org/ontology/TextualReknittings/Approval"/>
            <rdf:Description rdf:about="http://purl.org/ontology/TextualReknittings/Citation"/>
            <rdf:Description rdf:about="http://purl.org/ontology/TextualReknittings/Commentary"/>
            <rdf:Description rdf:about="http://purl.org/ontology/TextualReknittings/Disapproval"/>
            <rdf:Description rdf:about="http://purl.org/ontology/TextualReknittings/Important"/>
            <rdf:Description rdf:about="http://purl.org/ontology/TextualReknittings/Key-word"/>
            <rdf:Description rdf:about="http://purl.org/ontology/TextualReknittings/Trouble"/>
        </owl:members>
    </rdf:Description>
</rdf:RDF>



<!-- Generated by the OWL API (version 4.5.9.2019-02-01T07:24:44Z) https://github.com/owlcs/owlapi -->

